hax-lib/proof-libs/fstar/core/Core_models.Cmp.fst
@@ -97,7 +97,7 @@ let impl_1 (#v_T: Type0) (#[FStar.Tactics.Typeclasses.tcresolve ()] i0: t_Partia
     f_lt_pre
     =
     (fun
-        (#[FStar.Tactics.Typeclasses.tcresolve ()] i0: t_PartialOrd v_T v_T)
+        (#[FStar.Tactics.Typeclasses.tcresolve ()] i1: t_PartialOrd v_T v_T)
         (self: v_T)
         (y: v_T)
         ->
@@ -105,7 +105,7 @@ let impl_1 (#v_T: Type0) (#[FStar.Tactics.Typeclasses.tcresolve ()] i0: t_Partia
     f_lt_post
     =
     (fun
-        (#[FStar.Tactics.Typeclasses.tcresolve ()] i0: t_PartialOrd v_T v_T)
+        (#[FStar.Tactics.Typeclasses.tcresolve ()] i1: t_PartialOrd v_T v_T)
         (self: v_T)
         (y: v_T)
         (out: bool)
@@ -114,7 +114,7 @@ let impl_1 (#v_T: Type0) (#[FStar.Tactics.Typeclasses.tcresolve ()] i0: t_Partia
     f_lt
     =
     (fun
-        (#[FStar.Tactics.Typeclasses.tcresolve ()] i0: t_PartialOrd v_T v_T)
+        (#[FStar.Tactics.Typeclasses.tcresolve ()] i1: t_PartialOrd v_T v_T)
         (self: v_T)
         (y: v_T)
         ->
@@ -128,7 +128,7 @@ let impl_1 (#v_T: Type0) (#[FStar.Tactics.Typeclasses.tcresolve ()] i0: t_Partia
     f_le_pre
     =
     (fun
-        (#[FStar.Tactics.Typeclasses.tcresolve ()] i0: t_PartialOrd v_T v_T)
+        (#[FStar.Tactics.Typeclasses.tcresolve ()] i1: t_PartialOrd v_T v_T)
         (self: v_T)
         (y: v_T)
         ->
@@ -136,7 +136,7 @@ let impl_1 (#v_T: Type0) (#[FStar.Tactics.Typeclasses.tcresolve ()] i0: t_Partia
     f_le_post
     =
     (fun
-        (#[FStar.Tactics.Typeclasses.tcresolve ()] i0: t_PartialOrd v_T v_T)
+        (#[FStar.Tactics.Typeclasses.tcresolve ()] i1: t_PartialOrd v_T v_T)
         (self: v_T)
         (y: v_T)
         (out: bool)
@@ -145,7 +145,7 @@ let impl_1 (#v_T: Type0) (#[FStar.Tactics.Typeclasses.tcresolve ()] i0: t_Partia
     f_le
     =
     (fun
-        (#[FStar.Tactics.Typeclasses.tcresolve ()] i0: t_PartialOrd v_T v_T)
+        (#[FStar.Tactics.Typeclasses.tcresolve ()] i1: t_PartialOrd v_T v_T)
         (self: v_T)
         (y: v_T)
         ->
@@ -160,7 +160,7 @@ let impl_1 (#v_T: Type0) (#[FStar.Tactics.Typeclasses.tcresolve ()] i0: t_Partia
     f_gt_pre
     =
     (fun
-        (#[FStar.Tactics.Typeclasses.tcresolve ()] i0: t_PartialOrd v_T v_T)
+        (#[FStar.Tactics.Typeclasses.tcresolve ()] i1: t_PartialOrd v_T v_T)
         (self: v_T)
         (y: v_T)
         ->
@@ -168,7 +168,7 @@ let impl_1 (#v_T: Type0) (#[FStar.Tactics.Typeclasses.tcresolve ()] i0: t_Partia
     f_gt_post
     =
     (fun
-        (#[FStar.Tactics.Typeclasses.tcresolve ()] i0: t_PartialOrd v_T v_T)
+        (#[FStar.Tactics.Typeclasses.tcresolve ()] i1: t_PartialOrd v_T v_T)
         (self: v_T)
         (y: v_T)
         (out: bool)
@@ -177,7 +177,7 @@ let impl_1 (#v_T: Type0) (#[FStar.Tactics.Typeclasses.tcresolve ()] i0: t_Partia
     f_gt
     =
     (fun
-        (#[FStar.Tactics.Typeclasses.tcresolve ()] i0: t_PartialOrd v_T v_T)
+        (#[FStar.Tactics.Typeclasses.tcresolve ()] i1: t_PartialOrd v_T v_T)
         (self: v_T)
         (y: v_T)
         ->
@@ -191,7 +191,7 @@ let impl_1 (#v_T: Type0) (#[FStar.Tactics.Typeclasses.tcresolve ()] i0: t_Partia
     f_ge_pre
     =
     (fun
-        (#[FStar.Tactics.Typeclasses.tcresolve ()] i0: t_PartialOrd v_T v_T)
+        (#[FStar.Tactics.Typeclasses.tcresolve ()] i1: t_PartialOrd v_T v_T)
         (self: v_T)
         (y: v_T)
         ->
@@ -199,7 +199,7 @@ let impl_1 (#v_T: Type0) (#[FStar.Tactics.Typeclasses.tcresolve ()] i0: t_Partia
     f_ge_post
     =
     (fun
-        (#[FStar.Tactics.Typeclasses.tcresolve ()] i0: t_PartialOrd v_T v_T)
+        (#[FStar.Tactics.Typeclasses.tcresolve ()] i1: t_PartialOrd v_T v_T)
         (self: v_T)
         (y: v_T)
         (out: bool)
@@ -207,7 +207,7 @@ let impl_1 (#v_T: Type0) (#[FStar.Tactics.Typeclasses.tcresolve ()] i0: t_Partia
         true);
     f_ge
     =
-    fun (#[FStar.Tactics.Typeclasses.tcresolve ()] i0: t_PartialOrd v_T v_T) (self: v_T) (y: v_T) ->
+    fun (#[FStar.Tactics.Typeclasses.tcresolve ()] i1: t_PartialOrd v_T v_T) (self: v_T) (y: v_T) ->
       match
         f_partial_cmp #v_T #v_T #FStar.Tactics.Typeclasses.solve self y
         <:
